Polish STLC and needed infrastructure

LN/Singlesorted/Environment.v
@@ -1,10 +1,8 @@
 From Tealeaves Require Import
      Singlesorted.Classes.DecoratedTraversableModule
-     LN.Atom LN.Leaf LN.AtomSet LN.AssocList.
-     (*
-LN.Singlesorted.Operations
-LN.Singlesorted.Theory.
-*)
+     LN.Atom LN.Leaf LN.AtomSet LN.AssocList
+     LN.Singlesorted.Operations
+     LN.Singlesorted.Theory.
 
 Require Import Coq.Sorting.Permutation.
 
@@ -13,10 +11,14 @@ Import LN.AtomSet.Notations.
 Import LN.AssocList.Notations.
 Import Applicative.Notations.
 Import Sets.Notations.
+Import Applicative.Notations.
 Import DecoratedTraversableMonad.Notations.
 Open Scope list_scope.
 Open Scope set_scope.
 Open Scope tealeaves_scope.
+
+Definition scoped_env F `{Fmap F} `{Dist F} {A} :
+  F leaf -> alist A -> Prop := fun t γ => scoped F t (domset γ).
 
 (** * D-T functor instance for <<alist>> *)
 (******************************************************************************)
@@ -26,6 +28,7 @@ Section DecoratedTraversableFunctor_alist.
     `{Monoid W}.
 
   (** ** Traversable instance *)
+  (******************************************************************************)
   #[global] Instance Dist_alist : Dist (fun A => alist A)
     := Dist_compose.
 
@@ -33,6 +36,7 @@ Section DecoratedTraversableFunctor_alist.
     := Traversable_compose.
 
   (** ** Decorated instance *)
+  (******************************************************************************)
   #[global] Instance Decorate_alist :
     Decorate W (fun A => alist A)
     := Decorate_zero.
@@ -42,21 +46,30 @@ Section DecoratedTraversableFunctor_alist.
     := DecoratedFunctor_zero.
 
   (** ** DTM instance *)
+  (******************************************************************************)
   #[global] Instance DecoratedTraversableFunctor_alist :
     DecoratedTraversableFunctor W (fun A => alist A).
   Proof.
     constructor.
     typeclasses eauto.
     typeclasses eauto.
-    intros. ext l. induction l. unfold compose; cbn.
-    - now rewrite (app_pure_natural G).
-    - change (fun A => alist A) with (list ∘ prod atom).
-      unfold compose.
-      change (fun A => alist A) with (list ∘ prod atom).
-      unfold_ops @Dist_alist @Dist_compose.
-      unfold_ops @Fmap_alist @Fmap_compose.
-      unfold_ops @Decorate_alist @Decorate_zero.
-  Admitted.
+    intros.
+    unfold_ops @Dist_alist @Dist_compose.
+    unfold_ops @Fmap_alist @Fmap_compose.
+    unfold_ops @Decorate_alist @Decorate_zero.
+    reassociate <-.
+    change (fmap G (fmap (list ○ prod atom) ?f))
+      with (fmap (G ∘ list) (fmap (prod atom) f)).
+    #[local] Set Keyed Unification.
+    rewrite (dist_natural list).
+    reassociate -> on right.
+    rewrite (fun_fmap_fmap list).
+    rewrite (dist_natural (prod atom)).
+    reassociate -> on left. rewrite (fun_fmap_fmap list).
+    reassociate -> on left. rewrite (fun_fmap_fmap list).
+    rewrite (fun_fmap_fmap (prod atom)). reflexivity.
+    #[local] Unset Keyed Unification.
+  Qed.
 
 End DecoratedTraversableFunctor_alist.
 
@@ -65,14 +78,8 @@ End DecoratedTraversableFunctor_alist.
 Section DecoratedTraversableMonad_env.
 
   Context
-    `{DecoratedTraversableModule W F T}.
-
-  Instance: Monoid W.
-  inversion H. inversion dtmod_dec.
-  inversion drmod_functor. auto.
-  Qed.
-
-  Local Notation "'env' A" := (alist (F A)) (at level 50, no associativity).
+    `{DecoratedTraversableModule W F T}
+    `{! Monoid W}.
 
   Instance: DecoratedTraversableModule W ((list ∘ prod atom) ∘ F) T :=
     DecoratedTraversableModule_compose.
@@ -82,145 +89,298 @@ End DecoratedTraversableMonad_env.
 (** * Rewriting principles *)
 (******************************************************************************)
 
-(** ** Rewriting principles for <<tolist>> *)
-(******************************************************************************)
 Section env_rewriting_tolist.
 
   Context
-    `{DecoratedTraversableModule W F T}.
+    `{DecoratedTraversableModule nat (op := plus) (unit := 0) F T}.
 
-  Local Notation "'env' A" := (alist (F A)) (at level 50).
+  Definition env := ((list ∘ prod atom) ∘ F).
+
+  Instance: DecoratedTraversableModule nat env T :=
+    DecoratedTraversableModule_compose.
+
+  (** ** Rewriting principles for <<dist>> *)
+  (******************************************************************************)
+  Section dist_laws.
+
+    Context `{Applicative G}.
+
+    Lemma dist_env_spec : forall A (e : env (G A)),
+        dist env G e = dist list G (fmap list (dist (prod atom ∘ F) G) e).
+    Proof.
+      intros. unfold dist at 1, Dist_compose.
+      unfold dist at 1, Dist_alist, Dist_compose.
+      reassociate -> on left.
+      Set Keyed Unification.
+      now rewrite (fun_fmap_fmap list).
+      Unset Keyed Unification.
+    Qed.
+
+    Lemma dist_env_nil : forall A,
+        dist env G (nil : env (G A)) = pure G nil.
+    Proof.
+      reflexivity.
+    Qed.
+
+    Lemma dist_env_cons : forall A (x : atom) (t : F (G A)) (xs : env (G A)),
+        dist env G ((x, t) :: xs) =
+        pure G cons <⋆> (δ (prod atom ∘ F) G (x, t)) <⋆> (dist env G xs).
+    Proof.
+      reflexivity.
+    Qed.
+
+    Lemma dist_env_one : forall A (x : atom) (t : F (G A)),
+        dist env G (x ~ t) = pure G (η list) <⋆> dist (prod atom) G (x, dist F G t).
+    Proof.
+      intros. change (x ~ t) with ((x, t) :: nil).
+      rewrite dist_env_cons. rewrite dist_env_nil.
+      do 2 rewrite <- fmap_to_ap.
+      rewrite ap3. rewrite ap5.
+      reflexivity.
+    Qed.
+
+    Lemma dist_env_app : forall A (xs ys : env (G A)),
+        dist env G (xs ++ ys) =
+        pure G (app (A := atom * F A)) <⋆> dist env G xs <⋆> dist env G ys.
+    Proof.
+      intros. repeat rewrite dist_env_spec.
+      now simpl_list.
+    Qed.
+
+  End dist_laws.
+
+  (** ** Rewriting principles for <<fmap>> *)
+  (******************************************************************************)
+  Lemma fmap_env_nil : forall `(f : A -> B),
+      fmap env f (nil : env A) = nil.
+  Proof.
+    reflexivity.
+  Qed.
+
+  Lemma fmap_env_cons : forall `(f : A -> B) (x : atom) (t : F A) (xs : env A),
+      fmap env f ((x, t) :: xs) = (x, fmap F f t) :: fmap env f xs.
+  Proof.
+    reflexivity.
+  Qed.
+
+  Lemma fmap_env_one : forall `(f : A -> B) (x : atom) (t : F A),
+      fmap env f (x ~ t) = (x ~ fmap F f t).
+  Proof.
+    reflexivity.
+  Qed.
+
+  Lemma fmap_env_app : forall `(f : A -> B) (xs ys : env A),
+      fmap env f (xs ++ ys) = fmap env f xs ++ fmap env f ys.
+  Proof.
+    intros. change (fmap env f) with (fmap list (fmap (prod atom ∘ F) f)).
+    now simpl_list.
+  Qed.
+
+  (** ** Rewriting principles for <<sub>> *)
+  (******************************************************************************)
+  Lemma sub_env_spec : forall `(f : A -> T B) (e : env A),
+      sub env f e = fmap list (fmap (prod atom) (sub F f)) e.
+  Proof.
+    intros. unfold sub at 1, Sub_RightAction.
+    change (fmap env f) with (fmap list (fmap (prod atom ∘ F) f)).
+    Set Keyed Unification.
+    rewrite (fun_fmap_fmap list).
+    rewrite (fun_fmap_fmap (prod atom)).
+    reflexivity.
+    Unset Keyed Unification.
+  Qed.
+
+  Lemma sub_env_nil : forall `(f : A -> T B),
+      sub env f (nil : env A) = nil.
+  Proof.
+    reflexivity.
+  Qed.
+
+  Lemma sub_env_cons : forall `(f : A -> T B) (x : atom) (t : F A) (xs : env A),
+      sub env f ((x, t) :: xs) = (x, sub F f t) :: sub env f xs.
+  Proof.
+    reflexivity.
+  Qed.
+
+  Lemma sub_env_one : forall `(f : A -> T B) (x : atom) (t : F A),
+      sub env f (x ~ t) = (x ~ sub F f t).
+  Proof.
+    reflexivity.
+  Qed.
+
+  Lemma sub_env_app : forall `(f : A -> T B) (xs ys : env A),
+      sub env f (xs ++ ys) = sub env f xs ++ sub env f ys.
+  Proof.
+    intros. rewrite 3(sub_env_spec).
+    now simpl_list.
+  Qed.
+
+  (** ** Rewriting principles for <<tolist>> *)
+  (******************************************************************************)
+  Lemma tolist_env_spec : forall A (e : env A),
+      tolist env e = join list (fmap list (tolist F ∘ snd) e).
+  Proof.
+  Abort.
 
   Lemma tolist_env_nil : forall A,
-      tolist (fun A => env A) (nil : env A) = nil.
+      tolist env (nil : env A) = nil.
   Proof.
     reflexivity.
   Qed.
 
   Lemma tolist_env_cons : forall (x : atom) A (t : F A) (e : env A),
-      tolist (fun A => env A) ((x, t) :: e) =
-      tolist F t ++ tolist ((list ∘ prod atom) ∘ F) e.
+      tolist env ((x, t) :: e) =
+      tolist F t ++ tolist env e.
   Proof.
     intros. unfold_ops @Tolist_Traversable.
-    unfold compose. unfold_ops @Fmap_compose.
-    rewrite fmap_list_cons.
-    unfold_ops @Dist_compose @Dist_alist.
-    unfold compose; rewrite fmap_list_cons.
-    rewrite dist_list_cons. cbn.
-    unfold Dist_compose. unfold monoid_op, Monoid_op_app.
-    compose near e on left. rewrite (fun_fmap_fmap list).
-    unfold_ops @Fmap_alist @Fmap_compose.
-  Admitted.
+    change (fmap env ?f) with (fmap list (fmap (prod atom ∘ F) f)).
+    unfold compose. now rewrite fmap_list_cons.
+  Qed.
 
   Lemma tolist_env_one : forall (x : atom) A (t : F A),
-      (tolist (fun A => env A) (x ~ t)) = tolist F t.
+      (tolist env (x ~ t)) = tolist F t.
   Proof.
     intros. cbn. now rewrite (monoid_id_l).
   Qed.
 
   Lemma tolist_env_app : forall A (e1 e2 : env A),
-      tolist (fun A => env A) (e1 ++ e2) =
-      tolist (fun A => env A) e1 ++ tolist (fun A => env A) e2.
+      tolist env (e1 ++ e2) =
+      tolist env e1 ++ tolist env e2.
   Proof.
     intros. unfold_ops @Tolist_Traversable. unfold compose.
-    unfold_ops @Fmap_compose.
-  Admitted.
+    rewrite fmap_env_app.
+    now rewrite (dist_env_app).
+  Qed.
 
-End env_rewriting_tolist.
+  (** ** Rewriting principles for <<∈>> *)
+  (******************************************************************************)
+  Lemma in_env_nil : forall A (a : A),
+      a ∈ (nil : env A) = False.
+  Proof.
+    reflexivity.
+  Qed.
 
-(** ** Rewriting principles for LN operations *)
-(******************************************************************************)
-Section env_rewriting_ln.
+  Lemma in_env_cons : forall A (a : A) (x : atom) (t : F A) (e : env A),
+      a ∈ ((x, t) :: e : env A) <->
+      a ∈ t \/ a ∈ e.
+  Proof.
+    intros. unfold toset, Toset_Tolist.
+    unfold compose. rewrite tolist_env_cons.
+    simpl_list; simpl_set. easy.
+  Qed.
 
-  Context
-    `{DecoratedTraversableModule nat (op := plus) (unit0 := 0) F T}.
+  Lemma in_env_one : forall (x : atom) A (a : A) (t : F A),
+      a ∈ (x ~ t : env A) = a ∈ t.
+  Proof.
+    intros. cbn. now rewrite (monoid_id_l).
+  Qed.
 
-  Local Notation "'env' A" := (alist (F A)) (at level 50).
+  Lemma in_env_app : forall A (a : A) (e1 e2 : env A),
+      a ∈ (e1 ++ e2 : env A) <->
+      a ∈ e1 \/ a ∈ e2.
+  Proof.
+    intros. unfold toset, Toset_Tolist.
+    unfold compose. rewrite tolist_env_app.
+    now simpl_list; simpl_set.
+  Qed.
+
+  Lemma in_env_spec : forall A (a : A) (e : env A),
+      a ∈ (e : env A) <-> exists (x : atom) (t : F A), (x, t) ∈ (e : list (prod atom (F A))) /\ a ∈ t.
+  Proof.
+    intros. unfold toset at 1, Toset_Tolist.
+    split.
+    - unfold compose. induction e.
+      + intro hyp. inversion hyp.
+      + intro hyp. destruct a0 as [x t]. rewrite tolist_env_cons in hyp.
+        rewrite in_list_app in hyp. destruct hyp as [hyp | hyp].
+        { exists x, t. split. now left. auto. }
+        { specialize (IHe hyp). destruct IHe as [x' [t' rest]].
+          exists x', t'. split. now right. easy. }
+    - intros [x [t [hyp1 hyp2]]]. unfold compose.
+      rewrite <- in_iff_in_list. induction e.
+      + inversion hyp1.
+      + rewrite in_list_cons in hyp1. destruct hyp1 as [hyp1|hyp1].
+        { subst. rewrite in_env_cons. auto. }
+        { destruct a0 as [x' t'].
+          rewrite in_env_cons. right. auto. }
+  Qed.
 
   Import LN.Singlesorted.Operations.Notations.
 
   (** *** Rewriting lemmas for <<subst>> *)
-  Lemma subst_nil : forall (x : atom) (t : T leaf),
-      subst (fun A => env A) x t (nil : env leaf) = nil.
+  (******************************************************************************)
+  Lemma subst_env_nil : forall (x : atom) (t : T leaf),
+       ([] : env leaf) '{x ~> t} = [].
   Proof.
     intros. reflexivity.
   Qed.
 
-  Lemma subst_cons : forall (k : K) (x : atom) (t1 : F leaf) (t2 : T k leaf) (e : env leaf),
-      ((x, t1) :: e) '{k | x ~> t2} = (x, t1 '{k | x ~> t2}) :: (e '{k | x ~> t2}).
+  Lemma subst_env_cons : forall (x y : atom) (t1 : F leaf) (t2 : T leaf) (e : env leaf),
+      ((x, t1) :: e : env leaf) '{y ~> t2} =
+      (x, t1 '{y ~> t2}) :: e '{y ~> t2}.
   Proof.
     reflexivity.
   Qed.
 
-  Lemma subst_one : forall (k : K) (x y : atom) (t1 : F leaf) (t2 : T k leaf),
-      (x ~ t1) '{k | y ~> t2} = x ~ t1 '{k | y ~> t2}.
+  Lemma subst_env_one : forall (x y : atom) (t1 : F leaf) (t2 : T leaf),
+      (x ~ t1 : env leaf) '{y ~> t2} = (x ~ t1 '{y ~> t2}).
   Proof.
     reflexivity.
   Qed.
 
-  Lemma subst_app : forall (k : K) (x : atom) (t : T k leaf) (e1 e2 : env leaf),
-      (e1 ++ e2) '{k | x ~> t} = (e1 '{k | x ~> t}) ++ (e2 '{k | x ~> t}).
+  Lemma subst_env_app : forall (x : atom) (t : T leaf) (e1 e2 : env leaf),
+      (e1 ++ e2 : env leaf) '{x ~> t} =
+      e1 '{x ~> t} ++ e2 '{x ~> t}.
   Proof.
-    intros. unfold subst, bindk, mbind, Mbind_env.
-    now rewrite envmap_app.
-  Qed.
-
-  Lemma subst_app_one_l : forall (k : K) (x : atom) (t1 : F leaf) (t2 : T k leaf) (e : env leaf),
-      (x ~ t1 ++ e) '{k | x ~> t2} = x ~ t1 '{k | x ~> t2} ++ (e '{k | x ~> t2}).
-  Proof.
-    reflexivity.
-  Qed.
-
-  Lemma subst_app_one_2 : forall (k : K) (x : atom) (t1 : F leaf) (t2 : T k leaf) (e : env leaf),
-      (e ++ x ~ t1) '{k | x ~> t2} = (e '{k | x ~> t2}) ++ x ~ t1 '{k | x ~> t2}.
-  Proof.
-    intros. now rewrite subst_app.
+    intros. unfold subst. now rewrite sub_env_app.
   Qed.
 
   (** *** Rewriting lemmas for <<free>> *)
-  Lemma free_nil : forall (k : K) (x : atom) (t : T k leaf),
-      free (fun A => env A) k (nil : env leaf) = [].
+  (******************************************************************************)
+  Lemma free_nil : forall (x : atom) (t : T leaf),
+      free env (nil : env leaf) = [].
   Proof.
     reflexivity.
   Qed.
 
-  Lemma free_one : forall (k : K) (x : atom) (t : F leaf),
-      free (fun A => env A) k (x ~ t) = free F k t.
+  Lemma free_one : forall (x : atom) (t : F leaf),
+      free env (x ~ t) = free F t.
   Proof.
-    intros. unfold free, tolistk, compose.
-    now rewrite tolist_env_one.
+    intros. unfold free. now rewrite tolist_env_one.
   Qed.
 
-  Lemma free_cons : forall (k : K) (x : atom) (t : F leaf) (e : env leaf),
-      free (fun A => env A) k ((x, t) :: e) = free F k t ++ free (fun A => env A) k e.
+  Lemma free_cons : forall (x : atom) (t : F leaf) (e : env leaf),
+      free env ((x, t) :: e) = free F t ++ free env e.
   Proof.
-    intros. unfold free. unfold tolistk, compose, tolist, Tolist_env.
-    now rewrite List.bind_list_cons, filterk_app, List.bind_list_app.
+    intros. unfold free. rewrite tolist_env_cons.
+    now simpl_list.
   Qed.
 
-  Lemma free_app : forall (k : K) (e1 e2 : env leaf),
-      free (fun A => env A) k (e1 ++ e2) =
-      free (fun A => env A) k e1 ++ free (fun A => env A) k e2.
+  Lemma free_app : forall (e1 e2 : env leaf),
+      free env (e1 ++ e2) =
+      free env e1 ++ free env e2.
   Proof.
-    intros. unfold free, tolistk, tolist, Tolist_env, compose.
-    now rewrite List.bind_list_app, filterk_app, List.bind_list_app.
+    intros. unfold free. rewrite tolist_env_app.
+    now simpl_list.
   Qed.
 
+  (** *** Rewriting lemmas for <<∈ free>> *)
+  (******************************************************************************)
   Theorem in_free_iff :
-    forall (k : K) (Γ : env leaf) (x : atom),
-      x ∈ free (fun A => env A) k Γ  <-> exists (t : F leaf), t ∈ range Γ /\ x ∈ free F k t.
+    forall (Γ : env leaf) (x : atom),
+      x ∈ free env Γ  <-> exists (t : F leaf), t ∈ range Γ /\ x ∈ free F t.
   Proof.
     intros. rewrite (in_free_iff).
     setoid_rewrite (in_free_iff).
-    rewrite (inm_env_iff).
+    rewrite (in_env_spec).
     setoid_rewrite in_range_iff. split.
     - intros [y [t [? ?]]]. eauto.
     - intros [t [[y] ?]]. eauto.
   Qed.
 
   Theorem nin_free_iff :
-    forall (k : K) (Γ : env leaf) (x : atom),
-      ~ x ∈ free (fun A => env A) k Γ <-> forall (t : F leaf), t ∈ range Γ -> ~ x ∈ free F k t.
+    forall (Γ : env leaf) (x : atom),
+      ~ x ∈ free env Γ <-> forall (t : F leaf), t ∈ range Γ -> ~ x ∈ free F t.
   Proof.
     intros. alist induction Γ.
     - cbn. split; auto.
@@ -236,96 +396,57 @@ Section env_rewriting_ln.
         contradict contra. rewrite IHΓ. auto.
   Qed.
 
-  (** *** Rewriting lemmas for <<freeset>> *)
-  Open Scope set_scope.
-
-  Lemma freeset_nil : forall (k : K) (x : atom) (t : T k leaf),
-      freeset (fun A => env A) k (nil : env leaf) = ∅.
-  Proof.
-    reflexivity.
-  Qed.
-
-  Lemma freeset_one : forall (k : K) (x : atom) (t : F leaf),
-      freeset (fun A => env A) k (x ~ t) = freeset F k t.
-  Proof.
-    intros. unfold freeset. now rewrite free_one.
-  Qed.
-
-  Lemma freeset_cons : forall (k : K) (x : atom) (t : F leaf) (e : env leaf),
-      freeset (fun A => env A) k ((x, t) :: e) [=]
-              freeset F k t ∪ freeset (fun A => env A) k e.
-  Proof.
-    intros. unfold freeset. now rewrite free_cons, atoms_app.
-  Qed.
-
-  Lemma freeset_app : forall (k : K) (e1 e2 : env leaf),
-      freeset (fun A => env A) k (e1 ++ e2) [=]
-              freeset (fun A => env A) k e1 ∪ freeset (fun A => env A) k e2.
-  Proof.
-    intros. unfold freeset. now rewrite free_app, atoms_app.
-  Qed.
-
-End env_rewriting_lemmas.
-
-(** ** Reasoning principles for environments *)
-(******************************************************************************)
-Section env_theorems.
-
-  Context
-    `{SyntaxModule W F T}.
-
-  Local Notation "'env' A" := (alist (F A)) (at level 50).
-
-  Local Open Scope set_scope.
-
-  Theorem domset_subst : forall (e : env leaf) k x t,
-      domset e [=] domset (e '{ k | x ~> t}).
+  Theorem domset_subst : forall (e : env leaf) x t,
+      domset e [=] domset (e '{x ~> t}).
   Proof.
     intros. induction e.
     - reflexivity.
     - destruct a as [y u]. rewrite (domset_cons).
-      rewrite IHe. change_right ({{y}} ∪ domset (e '{ k | x ~> t})).
+      rewrite IHe. rewrite (subst_env_cons).
+      rewrite domset_cons.
       reflexivity.
   Qed.
 
-  Theorem uniq_subst : forall k (e : env leaf) x t,
-      uniq e <-> uniq (e '{ k | x ~> t}).
+  Theorem uniq_subst : forall (e : env leaf) x t,
+      uniq e <-> uniq (e '{x ~> t}).
   Proof.
-    intros. unfold subst. unfold bindk, mbind, Mbind_env.
-    now autorewrite with tea_rw_uniq.
+    intros. unfold subst.
+    rewrite sub_env_spec.
+    change (fmap list (fmap (prod atom) ?f)) with (fmap (list ∘ prod atom) f).
+    now rewrite uniq_fmap_iff.
   Qed.
 
-  Theorem binds_subst_env : forall k (e : env leaf) x t y u,
-      (y, u) ∈ (e '{k | x ~> t} : alist (F leaf)) <->
+  Theorem binds_subst_env : forall (e : env leaf) x t y u,
+      (y, u) ∈ (e '{x ~> t} : alist (F leaf)) <->
       exists u_inv : F leaf,
         (y, u_inv) ∈ (e : alist (F leaf))
-        /\ u_inv '{k | x ~> t} = u.
+        /\ u_inv '{x ~> t} = u.
   Proof.
-    intros. cbn. unfold subst, bindk, mbind, Mbind_env.
-    now rewrite in_envmap_iff.
-  Qed.
+    intros. cbn. unfold subst.
+    rewrite sub_env_spec.
+  Admitted.
 
-  Corollary binds_subst_env_mono : forall k (e : env leaf) x t (y : atom) (u : F leaf),
+  Corollary binds_subst_env_mono : forall (e : env leaf) x t (y : atom) (u : F leaf),
       (y, u) ∈ (e : alist (F leaf)) ->
-      (y, u '{k | x ~> t}) ∈ (e '{k | x ~> t} : list (atom * F leaf)).
+      (y, u '{x ~> t}) ∈ (e '{x ~> t} : list (atom * F leaf)).
   Proof.
     intros. rewrite binds_subst_env. eauto.
   Qed.
 
-  Theorem in_range_subst : forall k (e : env leaf) x t (u : F leaf),
-      u ∈ range (e '{k | x ~> t}) <->
+  Theorem in_range_subst : forall (e : env leaf) x t (u : F leaf),
+      u ∈ range (e '{x ~> t}) <->
       exists u_inv : F leaf,
         u_inv ∈ range (e : alist (F leaf))
-        /\ u_inv '{k |  x ~> t} = u.
+        /\ u_inv '{x ~> t} = u.
   Proof.
-    intros. cbn. unfold subst, bindk, mbind, Mbind_env.
+    intros. cbn. unfold subst. rewrite sub_env_spec.
     rewrite in_range_iff. setoid_rewrite in_range_iff.
-    setoid_rewrite in_envmap_iff. firstorder.
-  Qed.
+    setoid_rewrite in_envmap_iff.
+  Admitted.
 
-  Theorem in_freeset_iff : forall (k : K) (Γ : env leaf) (x : atom),
-      x ∈@ freeset (fun A => env A) k Γ  <->
-      exists (t : F leaf), t ∈ range Γ /\ x ∈@ freeset F k t.
+  Theorem in_freeset_iff : forall (Γ : env leaf) (x : atom),
+      x ∈@ freeset env Γ  <->
+      exists (t : F leaf), t ∈ range Γ /\ x ∈@ freeset F t.
   Proof.
     intros. rewrite <- free_iff_freeset.
     setoid_rewrite <- free_iff_freeset.
@@ -333,84 +454,69 @@ Section env_theorems.
   Qed.
 
   Theorem nin_freeset_iff :
-    forall (k : K) (Γ : env leaf) (x : atom),
-      ~ x ∈@ freeset (fun A => env A) k Γ  <-> forall (t : F leaf), t ∈ range Γ -> ~ x ∈@ freeset F k t.
+    forall (Γ : env leaf) (x : atom),
+      ~ x ∈@ freeset env Γ  <-> forall (t : F leaf), t ∈ range Γ -> ~ x ∈@ freeset F t.
   Proof.
     intros. setoid_rewrite <- free_iff_freeset.
     apply nin_free_iff.
   Qed.
 
-End env_theorems.
-
-(** ** Reasoning about <<scope>> *)
-(******************************************************************************)
-Definition scoped_env `{H : Index} F `{Tolist F} {A} :
-  K -> F leaf -> alist A -> Prop := fun k t γ => scoped F k t (domset γ).
-
-Section env_scope_theorems.
-
-  (** TODO : This choice of <<nat>> is unnecessarily specific but required for
-      using <<freeset_subst_upper_eq.>> *)
-
-  Context
-    `{SyntaxModule nat (monoid_op := plus) (monoid_unit := 0) F T}.
-
-  Theorem perm_scoped : forall A (t : F leaf) (γ1 γ2 : alist A) (k : K),
+  Theorem perm_scoped : forall A (t : F leaf) (γ1 γ2 : alist A),
       Permutation γ1 γ2 ->
-      scoped_env F k t γ1 ->
-      scoped_env F k t γ2.
+      scoped_env F t γ1 ->
+      scoped_env F t γ2.
   Proof.
     introv Hperm. unfold scoped_env, scoped. rewrite (perm_domset); eauto.
   Qed.
 
-  Theorem perm_scoped_iff : forall A (γ1 γ2 : alist A) (k : K) (t : F leaf),
+  Theorem perm_scoped_iff : forall A (γ1 γ2 : alist A) (t : F leaf),
       Permutation γ1 γ2 ->
-      scoped_env F k t γ1 <->
-      scoped_env F k t γ2.
+      scoped_env F t γ1 <->
+      scoped_env F t γ2.
   Proof.
     intros. assert (Permutation γ2 γ1) by now symmetry.
     split; eauto using perm_scoped.
   Qed.
 
-  Lemma weak_scoped_app_l : forall A k (t : F leaf) (γ1 γ2 : alist A),
-      scoped_env F k t γ1 ->
-      scoped_env F k t (γ1 ++ γ2).
+  Lemma weak_scoped_app_l : forall A (t : F leaf) (γ1 γ2 : alist A),
+      scoped_env F t γ1 ->
+      scoped_env F t (γ1 ++ γ2).
   Proof.
     intros. unfold scoped_env, scoped in *.
     autorewrite with tea_rw_dom. fsetdec.
   Qed.
 
-  Lemma weak_scoped_app_r : forall A k (t : F leaf) (γ1 γ2 : alist A),
-      scoped_env F k t γ2 ->
-      scoped_env F k t (γ1 ++ γ2).
+  Lemma weak_scoped_app_r : forall A (t : F leaf) (γ1 γ2 : alist A),
+      scoped_env F t γ2 ->
+      scoped_env F t (γ1 ++ γ2).
   Proof.
     intros. unfold scoped_env, scoped in *.
     autorewrite with tea_rw_dom. fsetdec.
   Qed.
 
-  Lemma stren_scoped : forall γ1 γ2 x t k,
-      scoped_env F k t (γ1 ++ x ~ tt ++ γ2) ->
-      ~ x ∈@ (freeset F k t) ->
-      scoped_env F k t (γ1 ++ γ2).
+  Lemma stren_scoped : forall γ1 γ2 x t,
+      scoped_env F t (γ1 ++ x ~ tt ++ γ2) ->
+      ~ x ∈@ (freeset F t) ->
+      scoped_env F t (γ1 ++ γ2).
   Proof.
     introv hyp hnotin. unfold scoped_env in *.
     (* todo : investigate why <<scoped>> needs to unfolded. *)
     unfold scoped in *. autorewrite with tea_rw_dom in *. fsetdec.
   Qed.
 
-  Lemma sub_scoped : forall γ1 γ2 x (t1 : F leaf) k (t2 : T k leaf) ,
-      scoped_env F k t1 (γ1 ++ x ~ tt ++ γ2) ->
-      scoped_env (T k) k t2 (γ1 ++ γ2) ->
-      scoped_env F k (subst F k x t2 t1) (γ1 ++ γ2).
+  Lemma sub_scoped : forall γ1 γ2 x (t1 : F leaf) (t2 : T leaf) ,
+      scoped_env F t1 (γ1 ++ x ~ tt ++ γ2) ->
+      scoped_env T t2 (γ1 ++ γ2) ->
+      scoped_env F (subst F x t2 t1) (γ1 ++ γ2).
   Proof.
     introv hyp1 hyp2. unfold scoped_env, scoped in *. autorewrite with tea_rw_dom in *.
-    etransitivity. apply freeset_subst_upper_eq. fsetdec.
+    etransitivity. apply freeset_subst_upper. fsetdec.
   Qed.
 
-  Lemma sub_scoped_1 : forall γ x (t1 : F leaf) k (t2 : T k leaf) ,
-      scoped_env F k t1 (γ ++ x ~ tt) ->
-      scoped_env (T k) k t2 γ ->
-      scoped_env F k (subst F k x t2 t1) γ.
+  Lemma sub_scoped_1 : forall γ x (t1 : F leaf) (t2 : T leaf) ,
+      scoped_env F t1 (γ ++ x ~ tt) ->
+      scoped_env T t2 γ ->
+      scoped_env F (subst F x t2 t1) γ.
   Proof.
     introv hyp1 hyp2. change_alist (γ ++ x ~ tt ++ []) in hyp1.
     change_alist (γ ++ []) in hyp2.
@@ -418,4 +524,4 @@ Section env_scope_theorems.
     eauto using sub_scoped.
   Qed.
 
-End env_scope_theorems.
+End env_rewriting_tolist.
