STLC/Theory.v
@@ -1,36 +1,40 @@
-Require Import TeaLeaves.Internal.
-Require Import TeaLeaves.Example.STLC.
-Require Import TeaLeaves.Backend.LocallyNamelessTheorems.
+From Tealeaves Require Export
+     Singlesorted.Theory.Product
+     LN.Leaf LN.Atom LN.AtomSet LN.AssocList
+     LN.Singlesorted.Environment
+     LN.Singlesorted.Operations
+     Singlesorted.Classes.DecoratedTraversableModule
+     STLC.Language.
 
-Import Functor.
-Import Monad.
-Import ListableFunctor.Notations.
-Import STLC.Notations.
-Import Monoid.Notations.
-Import LocallyNameless.LN.Monad.Notations.
+Export List.ListNotations.
+Open Scope list_scope.
+Export DecoratedTraversableMonad.Notations.
+Open Scope tealeaves_scope.
+Export LN.AtomSet.Notations.
+Open Scope set_scope.
+Export LN.AssocList.Notations.
 
-Notation "'freeset'" := LN.Monad.freeset.
-Notation "'locally_closed'" := LN.Monad.locally_closed.
-Notation "'δ'" := (DecoratedFunctor.read).
-Notation "'shift'" := ( DecoratedFunctor.shift).
+Import Operations.Notations.
+Import STLC.Language.Notations.
 
-
-Lemma inversion_var : forall (A : typ) (x : atom) (Γ : ctx),
-    Γ ⊢ (Var (F x)) : A -> binds x A Γ.
+(** * Inversion lemmas *)
+(******************************************************************************)
+Lemma inversion11 : forall (A : typ) (x : atom) (Γ : ctx),
+    Γ ⊢ (Var (Fr x)) : A -> (x, A) ∈ Γ.
 Proof.
   inversion 1; auto.
 Qed.
 
-Lemma inversion_var_b : forall (A : typ) (n : nat) (Γ : ctx),
-    Γ ⊢ (Var (B n)) : A -> False.
+Lemma inversion12 : forall (A : typ) (n : nat) (Γ : ctx),
+    Γ ⊢ (Var (Bd n)) : A -> False.
 Proof.
   inversion 1; auto.
 Qed.
 
-(** TODO: This is somewhat weak because L should really be (dom Γ) *)
-Lemma inversion_abs : forall (A B : typ) (e : term leaf) (Γ : ctx),
+(* This is somewhat weak because L should really be (dom Γ) *)
+Lemma inversion21 : forall (A B : typ) (e : term leaf) (Γ : ctx),
     (Γ ⊢ λ A ⋅ e : B) ->
-    exists C, B = A ⇒ C /\ exists L, forall (x : atom), ~ AtomSet.In x L -> Γ ++ x ~ A ⊢ e '(Var (F x)) : C.
+    exists C, B = A ⟹ C /\ exists L, forall (x : atom), ~ AtomSet.In x L -> Γ ++ x ~ A ⊢ e '(Var (Fr x)) : C.
 Proof.
   introv J.
   inversion J; subst.
@@ -38,172 +42,100 @@ Proof.
 Qed.
 
 (** Inversion principle for [abs] where we may assume the abstraction has arrow type *)
-Lemma inversion_abs' : forall (A B : typ) (e : term leaf) (Γ : ctx),
-    (Γ ⊢ λ A ⋅ e : A ⇒ B) ->
-    exists L, forall (x : atom), ~ AtomSet.In x L -> Γ ++ x ~ A ⊢ e '(Var (F x)) : B.
+Lemma inversion22 : forall (A B : typ) (e : term leaf) (Γ : ctx),
+    (Γ ⊢ λ A ⋅ e : A ⟹ B) ->
+    exists L, forall (x : atom), ~ AtomSet.In x L -> Γ ++ x ~ A ⊢ e '(Var (Fr x)) : B.
 Proof.
-  introv J. apply inversion_abs in J.
+  introv J. apply inversion21 in J.
   destruct J as [C [H1 H2]].
   assert (B = C) by (inversion H1; auto); subst.
   assumption.
 Qed.
 
-Lemma inversion_app : forall (A : typ) (Γ : ctx) (t1 t2 : term leaf),
+Lemma inversion3 : forall (A : typ) (Γ : ctx) (t1 t2 : term leaf),
     (Γ ⊢ [t1][t2] : A) ->
-    exists B, (Γ ⊢ t1 : B ⇒ A) /\ (Γ ⊢ t2 : B).
+    exists B, (Γ ⊢ t1 : B ⟹ A) /\ (Γ ⊢ t2 : B).
 Proof.
   introv J; inversion J; subst.
   exists A0. split; auto.
 Qed.
 
-Lemma in_abs_iff : forall (A : Type) t (x : A) (X : typ),
-    (x ∈ λ X ⋅ t) <-> x ∈ t.
-Proof.
-  intros.
-  reflexivity.
-Qed.
-
-Lemma in_freeset_abs_iff : forall (x : atom) (t : term leaf) (X : typ),
-    In x (freeset (λ X ⋅ t)) <-> In x (freeset t).
-Proof.
-  intros.
-  rewrite 2LN.in_freeset_F.
-  apply in_abs_iff.
-Qed.
-
-Lemma freeset_abs_spec: forall (t : term leaf) (X : typ),
-    freeset (λ X ⋅ t) [=] freeset t.
-Proof.
-  intros.
-  unfold AtomSet.Equal.
-  intros. apply in_freeset_abs_iff.
-Qed.
-
-Lemma in_read_abs_iff : forall t (l : leaf) (n : nat) (X : typ),
-    (n, l) ∈ δ (λ X ⋅ t) <-> (n - 1, l) ∈ δ t /\ n <> 0.
-Proof.
-  introv.
-  replace (δ (λ X ⋅ t) : term (nat * leaf)) with (λ X ⋅ shift 1 (δ t)).
-  - rewrite in_abs_iff.
-    (*
-    rewrite in_shift_minus; try typeclasses eauto.
-    split; intros [G1 G2]; split; auto; lia.
-  - cbn. unfold shift. unfold Term.shift.
-    f_equal. unfold fmap. *)
-Admitted.
-
-Lemma in_app_iff : forall (t1 t2 : term leaf) p,
-    p ∈ ([t1][t2]) <-> p ∈ t1 \/ p ∈ t2.
-Proof.
-  introv. cbn.
-  change (?x ++ ?y) with (x ● y).
-  rewrite List.fold_op.
-  reflexivity.
-Qed.
-
-Lemma in_freeset_app_iff : forall (t1 t2 : term leaf) (x : atom),
-    In x (freeset ([t1][t2])) <-> In x (freeset t1) \/ In x (freeset t2).
-Proof.
-  intros.
-  rewrite 3LN.in_freeset_F.
-  apply in_app_iff.
-Qed.
-
-Lemma freeset_app_spec : forall (t1 t2 : term leaf),
-    freeset ([t1][t2]) [=] freeset t1 ∪ freeset t2.
-Proof.
-  intros.
-  intros y. rewrite AtomSet.union_spec. apply in_freeset_app_iff.
-Qed.
-
-Lemma in_read_app_iff : forall (t1 t2 : term leaf) p,
-    p ∈ DecoratedFunctor.read ([t1][t2]) <-> p ∈ δ t1 \/ p ∈ δ t2.
-Proof.
-  introv. cbn.
-  change (?x ++ ?y) with (x ● y).
-  rewrite List.fold_op.
-  reflexivity.
-Qed.
-
+(** * Misc lemmas *)
+(******************************************************************************)
 Theorem j_ctx_wf : forall Γ (t : term leaf) (A : typ),
     Γ ⊢ t : A -> uniq Γ.
 Proof.
   introv J. induction J.
   - assumption.
-  - specialize_freshly H0. solve_uniq.
+  - specialize_freshly H0.
+    now autorewrite with tea_rw_uniq in H0.
   - assumption.
 Qed.
 
 Ltac gather_atoms ::=
-  let A := gather_atoms_with (fun x : AtomSet.t => x) in
-  let B := gather_atoms_with (fun x : atom => AtomSet.singleton x) in
-  let C := gather_atoms_with (fun x : term leaf => freeset x) in
-  let D := gather_atoms_with (fun x : env typ => domset x) in
+  let A := gather_atoms_with (fun s : AtomSet.t => s) in
+  let B := gather_atoms_with (fun x : atom => {{ x }}) in
+  let C := gather_atoms_with (fun t : term leaf => freeset term t) in
+  let D := gather_atoms_with (fun Γ : alist typ => domset Γ) in
   constr:(A ∪ B ∪ C ∪ D).
 
-Existing Instance LocallyNamelessModule_Monad.
-
 Theorem j_wf : forall Γ (t : term leaf) (A : typ),
-    Γ ⊢ t : A -> freeset t ⊆ domset Γ.
+    Γ ⊢ t : A -> scoped term t (domset Γ).
 Proof.
   introv J. induction J.
-  - apply binds_In in H0. cbn. fsetdec.
-  - rename H0 into IH.
-    rename H into premise.
-    specialize_freshly IH.
-    rewrite freeset_abs_spec.
-    assert (step1 : freeset t ⊆ freeset (t '(Var (F e)))).
-    { apply Theorems.freeset_open_lower. }
-    assert (step2 : forall x, In x (freeset t) -> In x (domset (Γ ++ e ~ A))).
+  - unfold scoped. rewrite term_freeset12.
+    unfold AtomSet.Subset; intro.
+    rewrite AtomSet.in_singleton_iff; intro; subst.
+    rewrite in_domset_iff. eauto.
+  - rename H0 into IH;
+      rename H into premise.
+    specialize_freshly IH. unfold scoped in *.
+    rewrite term_freeset2.
+    assert (step1 : freeset term t ⊆ freeset term (t '(Var (Fr e)))).
+    { apply Theory.freeset_open_lower. }
+    assert (step2 : forall x, x ∈@ (freeset term t) -> x ∈@ (domset (Γ ++ e ~ A))).
     { fsetdec. }
-    intros x xin.
-    assert (x <> e) by fsetdec.
-    specialize (step2 x xin).
-    rewrite dom_app in step2.
+    intros x xin. assert (x <> e) by fsetdec.
+    specialize (step2 x xin). rewrite domset_app in step2.
     cbn in step2. fsetdec.
-  - rewrite freeset_app_spec.
-    fsetdec.
+  - unfold scoped in *. rewrite term_freeset3. fsetdec.
 Qed.
-(*
-Lemma in_open_var : forall (p : nat * leaf) (x : atom) (t : term),
-    p ∈ δ (t '(Var (F x))) <-> exists (p1 : nat * leaf),
-      p1 ∈ δ t /\ ((is_opened p1 /\ snd p = F x) \/ (~ is_opened p1 /\ p = p1)).
-Proof.
-  intros.
-  rewrite in_dec_open_spec; try typeclasses eauto.
-  split.
-  - intros [p1 [p2 [G1 [G2 G3]]]].
-    exists p1. splits; auto.
-    destruct p1 as [p1_ctx [p1n | p1a]].
-    + simpl in *. right. split; auto.
 
-Admitted.
-*)
-
-Theorem lc_lam : forall (L : AtomSet.t) (t : term leaf) X,
-    (forall x : atom, ~ AtomSet.In x L -> locally_closed (t '(Var (F x)))) ->
-    locally_closed (λ X ⋅ t).
+Theorem is_bound_or_free_monotone : forall (k w1 w2 : nat) (l : leaf),
+    w1 < w2 ->
+    is_bound_or_free k (w1, l) ->
+    is_bound_or_free k (w2, l).
 Proof.
-  introv hyp.
-  unfold LN.Monad.locally_closed in *.
-  unfold LN.locally_closed in *.
-  rewrite ListableFunctor.fa_iso in *.
-  setoid_rewrite ListableFunctor.fa_iso in hyp.
-  intros [pn pl] pIn.
-  rewrite in_read_abs_iff in pIn.
-  destruct pIn as [pIn pNz].
+  cbn. unfold_ops @Monoid_op_plus.
+  introv Hlt Hyp. destruct l.
+  + easy.
+  + cbn in *. lia.
+Qed.
+
+Theorem lc_lam : forall (L : AtomSet.t) (t : term leaf) (X : typ),
+    (forall x : atom, ~ x ∈@ L -> locally_closed term (t '(Var (Fr x)))) ->
+    locally_closed term (λ X ⋅ t).
+Proof.
+  introv hyp1. unfold locally_closed, locally_closed_gap in *.
+  introv hyp2. rewrite term_ind22 in hyp2. destruct hyp2 as [m [hyp3 hyp4]].
+  subst. specialize_freshly hyp1.
+  destruct l.
+  - specialize (hyp1 m (Fr a)).
+    assert (lemma : (m, Fr a) ∈d t '( Var (Fr e))).
+    { admit. }
+    specialize (hyp1 lemma).
+    apply is_bound_or_free_monotone with (w1 := m). lia. auto.
+  - cbn in *. unfold_monoid.
+    specialize (hyp1 m (open_loc (Fr e) (m, (Bd n)))).
 Admitted.
 
 Theorem j_lc : forall Γ t A,
-    Γ ⊢ t : A -> locally_closed t.
+    Γ ⊢ t : A -> locally_closed term t.
 Proof.
   introv J. induction J.
-  - cbv; intuition.
+  - cbv. introv [hyp|]. now inversion hyp. easy.
   - pick fresh y excluding L and apply lc_lam; auto.
-  - unfold LN.Monad.locally_closed in *.
-    unfold LN.locally_closed in *.
-    cbn. rewrite List.fold_app.
-    firstorder.
+  - now rewrite term_lc3.
 Qed.
 
 Theorem weakening : forall Γ1 Γ2 Γ' (t : term leaf) (A : typ),
@@ -216,17 +148,13 @@ Proof.
   remember (Γ1 ++ Γ2) as Γrem.
   generalize dependent Γ2.
   induction J; intros; subst.
-  - apply j_var. solve_uniq.
-    analyze_binds_uniq H0.
-  - rename H0 into IH.
-    pick fresh y and apply j_abs.
-    specialize_cof IH y.
-    simpl_alist in *.
-    apply IH.
-    (** TODO I shouldn't have to do this manually *)
-    assert (LNotin : ~ AtomSet.In y (domset Γ')).
-    { fsetdec. }
-    solve_uniq. reflexivity.
+  - apply j_var. autorewrite with tea_rw_uniq tea_rw_disj in *.
+    rewrite disjoint_sym. preprocess. intuition.
+    simpl_list in *. intuition.
+  - rename H0 into IH. pick fresh y and apply j_abs.
+    specialize_cof IH y. simpl_alist in *.
+    apply IH; auto. autorewrite with tea_rw_disj in *.
+    splits; try easy. fsetdec.
   - eauto using j_app.
 Qed.
 
@@ -237,8 +165,9 @@ Proof.
   intros.
   rewrite <- (List.app_nil_r Γ1) in H.
   rewrite <- (List.app_nil_r (Γ1 ++ Γ2)).
-  rewrite app_assoc.
-  apply weakening; auto.
+  rewrite <- List.app_assoc.
+  apply weakening; auto. List.simpl_list.
+  eauto with tea_alist.
 Qed.
 
 Theorem substitution : forall Γ1 Γ2 (x : atom) (t u : term leaf) (A B : typ),
@@ -248,62 +177,55 @@ Theorem substitution : forall Γ1 Γ2 (x : atom) (t u : term leaf) (A B : typ),
 Proof.
   introv Jt Ju.
   specialize (j_ctx_wf (Γ1 ++ x~A ++ Γ2)); intro Hwf.
-  assert (locally_closed u).
-  { eauto using j_lc. }
-  remember (Γ1 ++ x ~ A ++ Γ2) as Γrem.
-  generalize dependent Γ2.
+  assert (locally_closed term u) by (eauto using j_lc).
+  remember (Γ1 ++ x ~ A ++ Γ2) as Γrem. generalize dependent Γ2.
   induction Jt; intros.
-  - Case "j_var".
-    cbn. destruct_eq.
-    + SCase "x = x0".
-      assert (A0 = A).
-      { subst. analyze_binds_uniq H1. }
+  - cbn. compare values x and x0.
+    + assert (A0 = A) by eauto using binds_mid_eq.
       subst; apply weakening_r; auto.
-      solve_uniq. solve_uniq.
-    + SCase "x <> x0".
-      subst. constructor.
-      solve_uniq. analyze_binds H1.
+      autorewrite with tea_rw_uniq in *. intuition.
+      autorewrite with tea_rw_uniq tea_rw_disj in *.
+      intuition.
+    + subst. constructor. eauto using uniq_remove_mid.
+      eauto using binds_remove_mid.
   - cbn. apply j_abs with (L := L ∪ domset Γ ∪ {{x}}).
-    intros_cof H1. change (join (fmap (subst_leaf x u) t)) with (t '{x ~> u}).
-    replace (Var (A := leaf)) with (term.ret (A := leaf)).
-    2:reflexivity.
+    intros_cof H1. change (right_action term (fmap term (subst_loc x u) t)) with (t '{x ~> u}).
+    change (Var (A := leaf)) with (η term (A := leaf)).
     rewrite <- subst_open_var.
     + simpl_alist in *. eapply H1.
-      (** TODO I shouldn't have to do this manually *)
-      assert (~ AtomSet.In e (domset Γ)).
-      { auto with set. }
-      solve_uniq. subst. simpl_alist. reflexivity.
+      * intros. subst. apply j_ctx_wf in H2. auto.
+      * subst. now simpl_alist.
     + fsetdec.
     + auto.
   - cbn. eauto using j_app.
 Qed.
 
-Corollary substitution_r : forall Γ (x : atom) (t u : term) (A B : typ),
+Corollary substitution_r : forall Γ (x : atom) (t u : term leaf) (A B : typ),
     (Γ ++ x ~ A ⊢ t : B) ->
     (Γ ⊢ u : A) ->
     (Γ ⊢ t '{x ~> u} : B).
 Proof.
   introv Jt Ju.
-  rewrite_alist (Γ ++ x ~ A ++ nil) in Jt.
-  rewrite_alist (Γ ++ nil).
+  change_alist (Γ ++ x ~ A ++ nil) in Jt.
+  change_alist (Γ ++ nil).
   eapply substitution; eauto.
 Qed.
 
-Inductive value : term -> Prop :=
+Inductive value : term leaf -> Prop :=
   | value_abs : forall X t,
       value (λ X ⋅ t).
 
-Inductive beta_step : term -> term -> Prop :=
-| beta_app_l : forall (t1 t2 t1' : term),
+Inductive beta_step : term leaf -> term leaf -> Prop :=
+| beta_app_l : forall (t1 t2 t1' : term leaf),
     beta_step t1 t1' ->
     beta_step ([t1][t2]) ([t1'][t2])
-| beta_app_r : forall (t1 t2 t2' : term),
+| beta_app_r : forall (t1 t2 t2' : term leaf),
     beta_step t2 t2' ->
     beta_step ([t1][t2]) ([t1][t2'])
-| beta_beta : forall (X : typ) (t u : term),
+| beta_beta : forall (X : typ) (t u : term leaf),
     beta_step ([λ X ⋅ t][u]) (t '(u)).
 
-Theorem subject_reduction_step : forall (t t' : term) Γ A,
+Theorem subject_reduction_step : forall (t t' : term leaf) Γ A,
     Γ ⊢ t : A -> beta_step t t' -> Γ ⊢ t' : A.
 Proof.
   intros t t' Γ A J step.
@@ -314,18 +236,18 @@ Proof.
   - intros; inversion step.
     + subst. apply j_app with (A := A); auto.
     + subst. apply j_app with (A := A); auto.
-    + subst. apply inversion_abs in J1.
+    + subst. apply inversion21 in J1.
       destruct J1 as [C [hyp1 [L hyp2]]].
       inversion hyp1; subst.
       specialize_freshly hyp2.
       assert (rw : t '(t2) = t '(Vf e) '{e ~> t2}).
-      { eapply subst_intro; try typeclasses eauto.
-        rewrite in_free_freeset. fsetdec. }
+      { erewrite open_spec_eq. reflexivity.
+        fsetdec. }
       rewrite rw. eapply substitution_r.
       exact hyp2. assumption.
 Qed.
 
-Theorem progress : forall (t : term) A,
+Theorem progress : forall (t : term leaf) A,
     nil ⊢ t : A -> value t \/ (exists t', beta_step t t').
 Proof.
   intros. remember [] as ctx.
